messageInvariantPrototypes/paxos/decentralizedMonotonic/readme.md
@@ -1,7 +1,0 @@
-# Readme
-
-Monotonic version of Decentralized Paxos.
-
-This is based on centralizedMonotonic Paxos.
-
-Want to compare if inductive invariants from centralizedMonotonic Paxos carry over here.
