messageInvariantPrototypes/paxos/decentralizedMonotonic_individualHistory/readme.md
@@ -1,0 +1,14 @@
+# Readme
+
+Monotonic version of Decentralized Paxos.
+
+This is based on centralizedMonotonic Paxos.
+
+Want to compare if inductive invariants from centralizedMonotonic Paxos carry over here.
+
+## Notes 7 Sept 2023
+
+In this version, each node maintains its own history.
+I think this does not work. Rather, the entire set of hosts should maintain a history. Otherwise, different host histories progress at different rates, and it becomes impossible to talk about a “consistent cut” of two host histories. Indeed, I am having trouble formalizing `AcceptorValidPromisedAndAccepted` as it requires talking about consistent historical states across nodes.
+
+Instead, if the whole hosts set maintains a history, then every property that is true in the non-monotonic version is true for every historical state in the monotonic version.
